asmrefine: improve debugging
Splits parts of step 4 of the SimplExport proof process, in order to
expose them to the test theory. Add some instructions on how to use
them.

Tags subgoals so that the user can identify which ones caused the
failure.

Consolidates ML setup code, and demarcates it to let uses ignore it.

proof/asmrefine/TestGraphRefine.thy
@@ -16,10 +16,80 @@ imports
   "SEL4SimplExport"
 begin
 
+\<comment>\<open> Name of the C function to investigate. \<close>
+ML \<open>
+val nm = "Kernel_C.dist_init"
+\<close>
+
 \<comment>\<open> Double-check we're reading the right graphlang file. \<close>
 ML \<open>
 writeln CFunDump_filename;
 val funs = ParseGraph.funs @{theory} CFunDump_filename
+\<close>
+
+\<comment>\<open>
+  These functions split up each part of "step 4", which is usually where
+  SimplExportAndRefine breaks.
+
+  Step 4 is roughly equivalent to:
+
+  debug_decompose_mem_goals ctxt
+    THEN_ALL_NEW debug_prove_mem_equality ctxt
+    THEN_ALL_NEW ProveSimplToGraphGoals.dest_ptr_add_assertion
+
+  `debug_decompse_mem_goals` lets you see what the actual memory update
+  goal looks like.
+
+  `debug_prove_mem_equality` let you "pause" in the middle of step 4, after
+  "prove_mem_equality" would normally error out because of a remaining
+  memory update goal.
+
+  Once paused, you can look for a simp rule that you
+  think will resolve the issue, then try adding it to
+  @{ML ProveSimplToGraphGoals.prove_mem_equality_unpack_simpset}.
+\<close>
+ML \<open>
+local
+  open ProveSimplToGraphGoals;
+in
+  val debug_decompose_mem_goals = decompose_mem_goals_init (K (K all_tac)) true;
+  fun debug_prove_mem_equality ctxt = DETERM o
+    (prove_mem_equality_unchecked ctxt
+    THEN_ALL_NEW SUBGOAL (fn (t, _) =>
+      (if exists_Const (fn (s, _) =>
+                 s = @{const_name store_word8}
+          orelse s = @{const_name store_word32}
+          orelse s = @{const_name store_word64}
+          orelse s = @{const_name heap_update}
+          orelse s = @{const_name heap_update_list}) t
+      then warning "prove_mem_equality: remaining mem upds. This would be a failure normally!"
+      else (); all_tac)))
+end
+\<close>
+
+\<comment>\<open>
+  A safe and easy way to attach a vacuous premise to your current goal,
+  with a message attached.
+\<close>
+definition Tag :: "'a \<Rightarrow> bool" where
+  "Tag data \<equiv> True"
+
+lemma tagI: "(Tag data \<Longrightarrow> P) \<Longrightarrow> P" by (simp add: Tag_def)
+
+ML \<open>
+fun tag_subgoals_tac ctxt idx: tactic =
+    let
+      val data = HOLogic.mk_string ("Subgoal " ^ Int.toString idx) |> Thm.cterm_of ctxt;
+      val typInst = ("'a", 0) |> rpair @{sort type} |> rpair @{ctyp string}
+      val termInst = ("data", 0) |> rpair @{typ string} |> rpair data;
+      val tagI = Thm.instantiate ([typInst], [termInst]) @{thm tagI};
+    in resolve0_tac [tagI] idx end
+\<close>
+
+\<comment>\<open>
+#####################################################################
+                     BEGIN SETUP BOILERPLATE
+#####################################################################
 \<close>
 
 ML \<open>
@@ -29,28 +99,17 @@ fun define_all funs = fold (fn s => let val s' = Long_Name.base_name s
   (Symtab.dest funs |> filter (fn (_, v) => #3 v <> NONE) |> map fst)
 \<close>
 
-ML \<open>
-val csenv = let
-    val the_csenv = CalculateState.get_csenv @{theory} "../c/build/$L4V_ARCH/kernel_all.c_pp" |> the
-  in fn () => the_csenv end
-\<close>
-
 consts
   encode_machine_state :: "machine_state \<Rightarrow> unit \<times> nat"
+
+context graph_refine_locale begin
 
 local_setup \<open>
   add_field_h_val_rewrites
   #> add_field_to_bytes_rewrites
   #> add_field_offset_rewrites
-\<close>
-
-context graph_refine_locale begin
-
-ML \<open>
-\<close>
-
-local_setup \<open>
-  add_globals_swap_rewrites @{thms kernel_all_global_addresses.global_data_mems}
+  #> add_globals_swap_rewrites @{thms kernel_all_global_addresses.global_data_mems}
+  #> define_graph_fun_short funs nm
 \<close>
 
 definition
@@ -71,6 +130,12 @@ lemma snd_snd_gs_new_frames_new_cnodes[simp]:
   by (simp_all add: gs_new_frames_def gs_new_cnodes_def gs_clear_region_def)
 
 ML \<open>
+val cfile = "../c/build/$L4V_ARCH/kernel_all.c_pp"
+
+val csenv = let
+    val the_csenv = CalculateState.get_csenv @{theory} cfile |> the
+  in fn () => the_csenv end
+
 val tacs = ProveSimplToGraphGoals.graph_refine_proof_tacs (csenv ())
     #> map snd
 val full_tac = ProveSimplToGraphGoals.graph_refine_proof_full_tac
@@ -83,20 +148,20 @@ val debug_step_tac = ProveSimplToGraphGoals.debug_step_tac
     (csenv ())
 \<close>
 
-\<comment>\<open> Name of the C function to investigate. \<close>
-ML \<open>
-val nm = "Kernel_C.merge_regions"
-\<close>
-
-local_setup \<open>define_graph_fun_short funs nm\<close>
-
 ML \<open>
 val hints = SimplToGraphProof.mk_hints funs @{context} nm
 val init_thm =
     SimplToGraphProof.simpl_to_graph_upto_subgoals funs hints nm @{context}
 \<close>
 
+\<comment>\<open>
+#####################################################################
+                      END SETUP BOILERPLATE
+#####################################################################
+\<close>
+
 declare [[show_types]]
+declare [[show_sorts]]
 declare [[goals_limit = 100]]
 
 \<comment>\<open>
@@ -106,43 +171,43 @@ schematic_goal "PROP ?P"
   apply (tactic \<open>resolve_tac @{context} [init_thm] 1\<close>)
 
   \<comment>\<open>
+    Mark each subgoal. Later, you can restrict your focus to the failing
+    initial goal.
+  \<close>
+  apply (tactic \<open>ALLGOALS (tag_subgoals_tac @{context})\<close>)
+
+(*
+  \<comment>\<open> `Goal.restrict x 1` selects subgoal `x`. \<close>
+  apply (tactic \<open>PRIMITIVE (Goal.restrict 102 1)\<close>)
+*)
+
+  \<comment>\<open>
     Apply the "all steps" debug tactic to every goal, but restore any
     unproven goals.
+
+    This can take a while for cases where there are lots of subgoals.
+    In that case, comment out this line and use the separate calls to
+    `debug_step_tac` below in order to find the failure.
   \<close>
   apply (all \<open>(solves \<open>tactic \<open>HEADGOAL (debug_tac @{context})\<close>\<close>)?\<close>)
 
-  \<comment>\<open> Lets us edit the next lines without re-running the above line. \<close>
+  \<comment>\<open> Lets us edit the following lines without re-running the above line. \<close>
   apply (tactic \<open>all_tac\<close>)
 
-  apply (tactic \<open>HEADGOAL (debug_step_tac @{context} 1)\<close>)
-  apply (tactic \<open>HEADGOAL (debug_step_tac @{context} 2)\<close>)
-  apply (tactic \<open>HEADGOAL (debug_step_tac @{context} 3)\<close>)
-  apply (tactic \<open>HEADGOAL (debug_step_tac @{context} 4)\<close>)
-  apply (tactic \<open>HEADGOAL (debug_step_tac @{context} 5)\<close>)
-  apply (tactic \<open>HEADGOAL (debug_step_tac @{context} 6)\<close>)
-  apply (tactic \<open>HEADGOAL (debug_step_tac @{context} 7)\<close>)
-  apply (tactic \<open>HEADGOAL (debug_step_tac @{context} 8)\<close>)
-  apply (tactic \<open>HEADGOAL (debug_step_tac @{context} 9)\<close>)
-  oops
-
-\<comment>\<open>
-  Extract a "working" part of the proof, to get a feel for what each step does.
-\<close>
-schematic_goal "PROP ?P"
-  apply (tactic \<open>resolve_tac @{context} [init_thm] 1\<close>)
-
-  \<comment>\<open> `Goal.restrict x 1` selects subgoal `x`. \<close>
-  apply (tactic \<open>PRIMITIVE (Goal.restrict 43 1)\<close>)
-
-  apply (tactic \<open>HEADGOAL (debug_step_tac @{context} 1)\<close>)
-  apply (tactic \<open>HEADGOAL (debug_step_tac @{context} 2)\<close>)
-  apply (tactic \<open>HEADGOAL (debug_step_tac @{context} 3)\<close>)
-  apply (tactic \<open>HEADGOAL (debug_step_tac @{context} 4)\<close>)
-  apply (tactic \<open>HEADGOAL (debug_step_tac @{context} 5)\<close>)
-  apply (tactic \<open>HEADGOAL (debug_step_tac @{context} 6)\<close>)
-  apply (tactic \<open>HEADGOAL (debug_step_tac @{context} 7)\<close>)
-  apply (tactic \<open>HEADGOAL (debug_step_tac @{context} 8)\<close>)
-  apply (tactic \<open>HEADGOAL (debug_step_tac @{context} 9)\<close>)
+  apply (tactic \<open>ALLGOALS (debug_step_tac @{context} 1)\<close>)
+  apply (tactic \<open>ALLGOALS (debug_step_tac @{context} 2)\<close>)
+  apply (tactic \<open>ALLGOALS (debug_step_tac @{context} 3)\<close>)
+  \<comment>\<open>
+    Step 4 is often where things break. You can use
+    @{ML "debug_decompose_mem_goals"} and @{ML "debug_prove_mem_equality"}
+    to investigate more closely - see their definitions for details.
+  \<close>
+  apply (tactic \<open>ALLGOALS (debug_step_tac @{context} 4)\<close>)
+  apply (tactic \<open>ALLGOALS (debug_step_tac @{context} 5)\<close>)
+  apply (tactic \<open>ALLGOALS (debug_step_tac @{context} 6)\<close>)
+  apply (tactic \<open>ALLGOALS (debug_step_tac @{context} 7)\<close>)
+  apply (tactic \<open>ALLGOALS (debug_step_tac @{context} 8)\<close>)
+  apply (tactic \<open>ALLGOALS (debug_step_tac @{context} 9)\<close>)
   oops
 
 end
